

University of California, Los Angeles  
Department of Statistics

Statistics C183/C283

Instructor: Nicolas Christou

**Exercise**

From *Options Futures and Other Derivatives* by John Hull, Prentice Hall 6th Edition, 2006.

The Black-Scholes-Merton formula for the value  $C$  of a European call option at time  $t$  and expiration time at time  $T$  is given by

$$C = S_0\Phi(d_1) - \frac{E}{e^{r(T-t)}}\Phi(d_2)$$

$$d_1 = \frac{\ln(\frac{S_0}{E}) + (r + \frac{1}{2}\sigma^2)(T-t)}{\sigma\sqrt{T-t}}$$

$$d_2 = \frac{\ln(\frac{S_0}{E}) + (r - \frac{1}{2}\sigma^2)(T-t)}{\sigma\sqrt{T-t}} = d_1 - \sigma\sqrt{T-t}$$

Answer the following questions:

1. Find  $\Phi'(d_1)$ .
2. Show that  $S_0\Phi'(d_1) = \frac{E}{e^{r(T-t)}}\Phi'(d_2)$ .
3. Find  $\frac{\partial d_1}{\partial S}$  and  $\frac{\partial d_2}{\partial S}$ .
4. Show that

$$\frac{\partial C}{\partial t} = -rEe^{-r(T-t)}\Phi(d_2) - S_0\Phi'(d_1)\frac{\sigma}{2\sqrt{T-t}}.$$

5. Show that  $\frac{\partial C}{\partial S} = \Phi(d_1)$ .
6. Show that  $C$  satisfies the Black-Scholes-Merton differential equation.
7. Show that  $C$  satisfies the boundary conditions for a European call option,  $C = \max[S-E, 0]$  as  $t \rightarrow T$ .

**Exercise 2**

Assume that a non-dividend-paying stock has an expected return of  $\mu$  and volatility of  $\sigma$ . A financial institution has just announced that it will trade a security that pays off a dollar amount equal to  $\ln(S_T)$  at time  $T$ , where  $S_T$  denotes the value of the stock price at time  $T$ . Answer the following questions:

- a. Use risk-neutral valuation to calculate the price of the security at time  $t$  in terms of the stock price at time  $T$ .
- b. Confirm that your price satisfies the Black-Scholes-Merton differential equation.

Answers

1. Since  $\Phi(d_i)$  is the cumulative probability that a standard normal random variable is less than  $d_1$ , i.e.,

$$P(Z \leq d_1) \text{ it follows that } \Phi'(d_1) = \frac{\partial \Phi(d_1)}{\partial d_1} = f(d_1) = \frac{1}{\sqrt{2\pi}} e^{-\frac{1}{2}d_1^2} = \frac{1}{\sqrt{2\pi}} e^{-\frac{1}{2} \left( \frac{\ln(\frac{S_0}{E}) + (r + \frac{1}{2}\sigma^2)(T-t)}{\sigma\sqrt{T-t}} \right)^2}.$$

2. Because

$$d_2 = \frac{\ln(\frac{S_0}{E}) + (r - \frac{1}{2}\sigma^2)(T-t)}{\sigma\sqrt{T-t}} = d_1 - \sigma\sqrt{T-t},$$

it follows that  $d_1 = d_2 + \sigma\sqrt{T-t}$ . Therefore,

$$\begin{aligned} \Phi'(d_1) &= \frac{\partial \Phi(d_1)}{\partial d_1} = f(d_1) = f(d_2 + \sigma\sqrt{T-t}) \\ &= \frac{1}{\sqrt{2\pi}} e^{-\frac{1}{2}(d_2 + \sigma\sqrt{T-t})^2} = \frac{1}{\sqrt{2\pi}} e^{-\frac{1}{2}(d_2^2 + 2d_2\sigma\sqrt{T-t} + \sigma^2(T-t))} \\ &= \frac{1}{\sqrt{2\pi}} e^{-\frac{1}{2}d_2^2} \times e^{-d_2\sigma\sqrt{T-t} - \frac{1}{2}\sigma^2(T-t)} = \Phi'(d_2) \times e^{-\frac{1}{2}d_2^2} \times e^{-d_2\sigma\sqrt{T-t} - \frac{1}{2}\sigma^2(T-t)} \end{aligned}$$

but

$$\begin{aligned} d_2 &= \frac{\ln(\frac{S_0}{E}) + (r - \frac{1}{2}\sigma^2)(T-t)}{\sigma\sqrt{T-t}}, \text{ therefore} \\ \Phi'(d_1) &= \Phi'(d_2) \times e^{-\sigma \left[ \frac{\ln(\frac{S_0}{E}) + (r - \frac{1}{2}\sigma^2)(T-t)}{\sigma\sqrt{T-t}} \right] \sqrt{T-t} - \frac{1}{2}\sigma^2(T-t)} \\ &= \Phi'(d_2) \times e^{-\ln \frac{S_0}{E} - r(T-t)} = \Phi'(d_2) \times e^{\ln \frac{E}{S_0} - r(T-t)} \\ &= \Phi'(d_2) \times \frac{E}{S_0} e^{-r(T-t)}. \text{ It follows that} \\ S_0 \Phi'(d_1) &= E e^{-r(T-t)} \Phi'(d_2). \end{aligned}$$

3. Use  $d_1 = \frac{\ln(\frac{S_0}{E}) + (r + \frac{1}{2}\sigma^2)(T-t)}{\sigma\sqrt{T-t}}$  and write it as  $d_1 = \frac{\ln S_0 + \ln E + (r + \frac{1}{2}\sigma^2)(T-t)}{\sigma\sqrt{T-t}}$ .

Therefore,  $\frac{\partial d_1}{\partial S} = \frac{1}{S\sigma\sqrt{T-t}}$ . Similarly, because  $d_2 = d_1 - \sigma\sqrt{T-t}$ , it follows that  $\frac{\partial d_2}{\partial S} = \frac{\partial d_1}{\partial S} = \frac{1}{S\sigma\sqrt{T-t}}$ .

4. Use the B-S-M formula:

$$\begin{aligned} C &= S_0 \Phi(d_1) - \frac{E}{e^{r(T-t)}} \Phi(d_2) \\ \frac{\partial C}{\partial t} &= S \Phi'(d_1) \frac{\partial d_1}{\partial t} - \frac{rE\Phi(d_2)}{e^{r(T-t)}} - \frac{E}{e^{r(T-t)}} \Phi'(d_2) \frac{\partial d_2}{\partial t} \\ \text{From (2) } S_0 \Phi'(d_1) &= E e^{-r(T-t)} \Phi'(d_2), \text{ therefore} \\ \frac{\partial C}{\partial t} &= S \Phi'(d_1) \frac{\partial d_1}{\partial t} - \frac{rE\Phi'(d_2)}{e^{r(T-t)}} - S \Phi'(d_1) \frac{\partial d_2}{\partial t} \\ &= S \Phi'(d_1) \left( \frac{\partial d_1}{\partial t} - \frac{\partial d_2}{\partial t} \right) - \frac{rE\Phi'(d_2)}{e^{r(T-t)}}. \end{aligned}$$

$$\text{But } d_1 - d_2 = \sigma\sqrt{T-t}, \text{ which means } \frac{\partial d_1}{\partial t} - \frac{\partial d_2}{\partial t} = -\frac{\sigma}{\sqrt{T-t}}.$$

$$\text{Finally, } \frac{\partial C}{\partial t} = -rE e^{-r(T-t)} \Phi(d_2) - S_0 \Phi'(d_1) \frac{\sigma}{2\sqrt{T-t}}, \text{ which is a decreasing function of } t.$$

5. This is the hedge ratio  $\frac{\partial C}{\partial S} = \Phi(d_1)$ . Again, begin with the formula for  $C$ .

$$\begin{aligned}
C &= S_0\Phi(d_1) - \frac{E}{e^{r(T-t)}}\Phi(d_2) \\
\frac{\partial C}{\partial S} &= \Phi(d_1) + S\Phi'(d_1)\frac{\partial d_1}{\partial S} - \frac{E}{e^{r(T-t)}}\Phi'(d_2)\frac{\partial d_2}{\partial S} \\
\text{From (2) } S_0\Phi'(d_1) &= \frac{E}{e^{r(T-t)}}\Phi'(d_2) \\
\text{From (3) } \frac{\partial d_1}{\partial S} &= \frac{\partial d_2}{\partial S} = \frac{1}{S\sigma\sqrt{T-t}}. \\
\text{Therefore } \frac{\partial C}{\partial S} &= \Phi(d_1) + \frac{E}{e^{r(T-t)}}\Phi'(d_2)\frac{1}{S\sigma\sqrt{T-t}} - \frac{E}{e^{r(T-t)}}\Phi'(d_2)\frac{1}{S\sigma\sqrt{T-t}} = \Phi(d_1).
\end{aligned}$$

6.  $C$  satisfies the B-S-M formula.

From (5) and (3) it follows that  $\frac{\partial^2 C}{\partial S^2} = \Phi'(d_1)\frac{\partial d_1}{\partial S} = \Phi'(d_1)\frac{1}{S\sigma\sqrt{T-t}}$ . Therefore,

$$\frac{\partial C}{\partial t} \text{ (from (3))} + rS\frac{\partial C}{\partial S} \text{ (from (5))} + \frac{1}{2}S^2\frac{\partial^2 C}{\partial S^2} = rC.$$

7. Examine what happens as  $t \rightarrow T$ .

If  $S > E$  then  $d_1 \rightarrow \infty$  and  $d_2 \rightarrow \infty$  and therefore  $\Phi(d_1) \rightarrow 1$  and  $\Phi(d_2) \rightarrow 1$ .

In this case  $C \rightarrow S - E$ .

If  $S < E$  then  $d_1 \rightarrow -\infty$  and  $d_2 \rightarrow -\infty$  and therefore  $\Phi(d_1) \rightarrow 0$  and  $\Phi(d_2) \rightarrow 0$ .

Now,  $C \rightarrow 0$ .

We see that as  $t \rightarrow T$ ,  $C \rightarrow \max(S - E, 0)$ .